define product semantics

KLR/Semantics/SmallStep.lean
@@ -10,8 +10,7 @@ Authors: Markus de Medeiros
 class SmallStep (Pgm State Val : Type _) where
   step : Pgm × State → Pgm × State → Prop
   to_value : Pgm × State → Option Val
-  value_stuck : (¬ to_value c = .none) → ¬ step c c'
-
+  value_stuck : (to_value c).isSome → ¬∃ c', step c c'
 
 section SmallStep
 
@@ -22,6 +21,32 @@ This implies a trace where no intermediate state is a value, and is probably not
 inductive stepExactN : Nat → Pgm × State → Pgm × State → Prop where
 | step0 : stepExactN 0 c c
 | stepS : SmallStep.step Val c c' → stepExactN n c' c'' → stepExactN n.succ c c''
+
+theorem stepExactN_1_iff_step : stepExactN Pgm State Val 1 (p, s) (p', s') ↔ I.step (p, s) (p', s') := by
+  refine ⟨?_, (stepExactN.stepS · stepExactN.step0)⟩
+  rintro (_|⟨_,_|_⟩)
+  trivial
+
+theorem step_none (H : SmallStep.step Val (p2', s2') (p2, s2)) :
+    (SmallStep.to_value (Pgm := Pgm) (State := State) (Val := Val) (p2', s2')).isNone := by
+  suffices ¬(SmallStep.to_value (Val := Val) (p2', s2')).isSome by
+    generalize HX : (SmallStep.to_value (Val := Val) (p2', s2')) = X
+    rw [HX] at this
+    cases X <;> simp_all
+  intro H'
+  apply (SmallStep.value_stuck H')
+  exists (p2, s2)
+
+theorem stepExactN_succ_some {n : Nat} (H : stepExactN Pgm State Val n.succ (p2', s2') (p2, s2)) :
+    (SmallStep.to_value (Val := Val) (p2', s2')).isNone := by
+  rcases H with (_|_)
+  suffices ¬(SmallStep.to_value (Val := Val) (p2', s2')).isSome by
+    generalize HX : (SmallStep.to_value (Val := Val) (p2', s2')) = X
+    rw [HX] at this
+    cases X <;> simp_all
+  intro H
+  apply (SmallStep.value_stuck H)
+  rename_i c _ _; exists c
 
 def stuck (c : Pgm × State) : Prop := ∀ c', ¬ SmallStep.step Val c c'
 
@@ -38,8 +63,7 @@ def is_value? (c : Pgm × State) : Prop := ¬ (SmallStep.to_value (Val := Val) c
 
 /-- For the first n steps of execution, all stuck states are values. -/
 def safeN (n : Nat) : Pgm × State → Prop :=
-  sorry
-  -- satN _ _ _ n (is_value? Pgm State Val) -- what is going on here...
+  satN (I := I) _ _ _ n (is_value? Pgm State Val)
 
 -- theorem safeN.mono (c : Pgm × State) (Hn : n ≤ n') (Hs : safeN _ _ n' c) : safeN _ _ n c := by
 --   revert n
@@ -50,6 +74,51 @@ def safeN (n : Nat) : Pgm × State → Prop :=
 --   sorry
 
 /-- For all terminating executions, all stuck states are values. -/
-def safe (c : Pgm × State) : Prop := ∀ n, safeN _ _ n c
+def safe (c : Pgm × State) : Prop := ∀ n, safeN (I := I) _ _ _ n c
 
 end SmallStep
+
+
+section Product
+
+/- Lift a small-step semantics to product programs -/
+
+variable {Pgm State Val : Type _} [I : SmallStep Pgm State Val]
+
+/-- Stepping relation for product programs. -/
+inductive Product.step : (Pgm × Pgm) × State × State → (Pgm × Pgm) × State × State → Prop where
+| step_l : SmallStep.step Val (p1, s1) (p1', s1') → step ((p1, p2), (s1, s2)) ((p1, p2'), (s1, s2'))
+| step_r : SmallStep.step Val (p2, s2) (p2', s2') → step ((p1, p2), (s1, s2)) ((p1, p2'), (s1, s2'))
+
+def Product.to_value : (Pgm × Pgm) × State × State → Option (Val × Val)
+| ((p1, p2), (s1, s2)) =>
+  match I.to_value (p1, s1), I.to_value (p2, s2) with
+  | .some v1, .some v2 => .some (v1, v2)
+  | _, _ => .none
+
+instance Product.is_SmallStep : SmallStep (Pgm × Pgm) (State × State) (Val × Val) where
+  step := Product.step (I := I)
+  to_value := Product.to_value
+  value_stuck {c} := by
+    rcases c with ⟨⟨p1, p2⟩, ⟨s1, s2⟩⟩
+    simp only [to_value]
+    split
+    · rename_i v1 v2 Hv1 Hv2
+      intro _
+      rintro ⟨c, Hc⟩
+      cases Hc
+      · rename_i _ Hstep
+        have Hstep' := step_none Pgm State Val Hstep
+        simp [Hv1] at Hstep'
+      · rename_i _ Hstep
+        have Hstep' := step_none Pgm State Val Hstep
+        simp [Hv2] at Hstep'
+    · simp
+
+/-- Lift a relation on final values to a relation on program terms, which is trivially true for all non-value terms. -/
+def lift_rel (R : Val × State → Val × State → Prop) (p1 p2 : Pgm × State) : Prop :=
+  match SmallStep.to_value p1, SmallStep.to_value p2 with
+  | some v1, some v2 => R ⟨v1, p1.2⟩ ⟨v2, p2.2⟩
+  | _, _ => True
+
+end Product
